refactor: Explicitly track which (linear) variables have become stale (#29)
This PR refactors a context to be a list of optional types, where a particular entry being none means that the corresponding variable was linear and has been used already, thus implementing #21.

This replaces the previous mechanism, where linear variables were completely erased from the context, which in turn meant that the De Bruijn indices of linear variable were getting reused and the corresponding values in an environment had to be erased.

With the new notion of context, we can keep the old values around in the environment, which will be necessary if we get around to stating an equation lemma.

An alternative design could be to tag each type in a context with a "Staleness" value (which is just an enum which is either live or stale), such that we don't have to remove types from the context at all, we just mark the variables as used. This might be necessary, as currently the value of a stale variable does get kept in an environment when the variable is used, but it's type information is no longer tracked in the well-typedness of the environment. With the explicit Staleness tags, we can require that even stale values in an environment still have the right value.

EffectSSA/Semantics/Environment.lean
@@ -34,6 +34,14 @@ inductive Ty.TVal : τ.Typ → Type where
 def Ty.Val : Type := Σ t, τ.TVal t
 -- FIXME: maybe `Ty.Val` ought to be a structure? We'll evaluate later.
 
+/--
+An environment maps variables to values.
+
+Note that environments do *not* distinguish between live or dead variables,
+which means that our semantics will not throw an error when linearity conditions
+are violated. This is fine; well-formed guarantees the absence of (type) errors,
+but the abscense of errors does not guarantee well-formedness
+-/
 structure Semantics.Environment τ [MemoryModel τ] where
   ofList :: toList : List τ.Val
 
@@ -62,6 +70,12 @@ instance : Coe (τ.TVal .eff) (Trace τ) where coe := fun (.eff e) => e
 instance : Coe (τ.TVal .ptr) τ.Ptr where coe := fun (.ptr p) => p
 instance : Coe (τ.TVal <| .data t) (τ.DVal t) where coe := fun (.data x) => x
 end TVal
+
+noncomputable
+instance : Inhabited (τ.TVal .eff) where default := .eff default
+
+noncomputable
+instance : Inhabited τ.Val := ⟨.eff, default⟩
 
 /-- Coerce a statically typed value into a dynamically typed value. -/
 @[grind] abbrev TVal.toVal : τ.TVal t → τ.Val := (⟨t, ·⟩)
@@ -122,7 +136,7 @@ def getData? (env : Environment τ) (v : Var) (t : τ.DType) : Option (τ.DVal t
 /--
 `env.snoc x` adds a new variable to environment `env` assigning value `x` to it.
 -/
-def snoc (x : τ.Val) (env : Environment τ) : Environment τ :=
+def snoc (env : Environment τ) (x : τ.Val) : Environment τ :=
   ⟨env.toList.cons x⟩
 
 /-! #### Environment Modification -/
@@ -177,6 +191,13 @@ end Semantics.Environment
 -/
 namespace Semantics.Environment
 
-@[grind =]
-def WellTyped (Γ : Context τ) (env : Environment τ) : Prop :=
-  ∀ (v : Var) (t : τ.Typ), Γ[v]? = some t ↔ (env.getAs? v t).isSome
+/--
+An environment `env` is welltyped w.r.t. context `Γ` when:
+* `env` has as many values as `Γ` has variables (including stale variables), and
+* all _live_ variables of `Γ` have a value, of the appropriate type, assigned by `env`.
+
+Note that the values which `env` assigns to _stale_ variables are not constrained.
+-/
+@[grind, grind cases] structure WellTyped (Γ : Context τ) (env : Environment τ) : Prop where
+  length_eq : env.size = Γ.size
+  isSome_getAs? : ∀ (v : Var) (t : τ.Typ), Γ[v]? = some t → (env.getAs? v t).isSome
