EffectSSA/Types/Context/Basic.lean
@@ -18,10 +18,14 @@ namespace EffectSSA
 -/
 
 /--
-A `Context τ` is a mapping from `n` variables to their types.
+A `Context τ` is a mapping from variables to (optional) types.
+
+A linear variable, when used, will be replaced by a `none` to indicate that the
+corresponding variable is no longer available. By keeping the entry in the
+context, we prevent having to reuse variable indices.
 -/
 structure Context (τ : Ty) where
-  ofList :: toList : List τ.Typ
+  ofList :: toList : List (Option τ.Typ)
 
 /-!
 ## Definitions
@@ -31,16 +35,29 @@ structure Context (τ : Ty) where
 @[grind =]
 abbrev Context.size (Γ : Context τ) : Nat := Γ.toList.length
 
-def Var.InBounds (Γ : Context τ) (v : Var) : Prop := v.toNat < Γ.size
+/--
+`Γ.get? v` returns the type assigned to variable `v`,
+returning `none` when `v` is either out of bounds for `Γ`,
+or when `v` is "stale", meaning that the corresponding entry in `Γ` is `none`.
+
+The preferred spelling of `Γ.get? v` is `Γ[v]?`.
+-/
+protected def Context.get? (Γ : Context τ) (v : Var) : Option τ.Typ :=
+  Γ.toList[v.toNat]?.join
+
+/--
+`v.LiveIn Γ` holds when the index of variable `v` is in bounds of context `Γ`,
+and is _live_, i.e., has a type assigned to it in `Γ`.
+-/
+def Var.LiveIn (Γ : Context τ) (v : Var) : Prop :=
+  (Γ.get? v).isSome
 
 namespace Context
 
-/--
-We write `Γ[v]` to indicate the type that context `Γ` assigned to variable `v`.
--/
-instance : GetElem? (Context τ) (Var) (τ.Typ) (fun Γ v => v.InBounds Γ) where
-  getElem Γ v _ := Γ.toList[v.toNat]
-  getElem? Γ v := Γ.toList[v.toNat]?
+/-- `Γ[v]?` is an alias for `Γ.get? v` -/
+instance : GetElem? (Context τ) (Var) τ.Typ (fun Γ v => v.LiveIn Γ) where
+  getElem Γ v h := (Γ.get? v).get h
+  getElem? Γ v  := Γ.get? v
 
 /--
 `∅` is the empty context.
@@ -48,42 +65,38 @@ instance : GetElem? (Context τ) (Var) (τ.Typ) (fun Γ v => v.InBounds Γ) wher
 instance : EmptyCollection (Context τ) where emptyCollection := ⟨[]⟩
 
 /--
-`Γ <: t` is the context `Γ` expanded with a new variable of type `t`.
+`Γ <: t` expands the context `Γ` with a new (live) variable of type `t`.
 -/
 def snoc (Γ : Context τ) (t : τ.Typ) : Context τ :=
-  ⟨Γ.toList.cons t⟩
+  ⟨Γ.toList.cons (some t)⟩
 @[inherit_doc] infixl:67 " <: " => snoc
+
+/--
+`Γ.snocStale` expands the context `Γ` with a new stale variable.
+
+This should probably not be used by users of the API; instead, it should only
+show up in the intermediate state of a proof.
+-/
+def snocStale (Γ : Context τ) : Context τ :=
+  ⟨Γ.toList.cons none⟩
 
 /--
 A context is unrestricted if *all* contained types are unrestricted.
 -/
 def isUnrestricted (Γ : Context τ) : Prop :=
-  ∀ (v : Var), (h : v.InBounds Γ) → Γ[v].isUnrestricted
-
-/--
-Unrestrictedness of a context is decidable.
--/
-instance {Γ : Context τ} : Decidable (isUnrestricted Γ) :=
-  decidable_of_iff (
-      List.range Γ.size |>.attach |>.all fun ⟨x, hx⟩ =>
-        let v := Var.ofNat x
-        have : v.InBounds Γ := by simpa using hx
-        Γ[v].isUnrestricted
-      ) <| by
-    simp [isUnrestricted, Var.InBounds]
-    grind
-
+  ∀ (v : Var) {t}, Γ[v]? = some t → t.isUnrestricted
 
 /-! ### vars -/
 
 /--
-`Γ.eraseVar v` removes variable `v` from the context.
+`Γ.eraseVar v` marks variable `v` as stale, or returns `Γ` unchanged if `v` is
+not in bounds of `Γ`.
 -/
 def eraseVar (v : Var) (Γ : Context τ) : Context τ :=
-  ⟨Γ.toList.eraseIdx v.toNat⟩
+  ⟨Γ.toList.set v.toNat none⟩
 
 /--
-`Γ.eraseVars vs` removes a list of variables `vs` from the context,
+`Γ.eraseVars vs` marks a list of variables `vs` as stale,
 optionally starting the first variable at an index other than 0.
 
 For example:
@@ -91,7 +104,8 @@ For example:
 * `[α, β, γ].eraseVars [0]    = [β, γ]`
 * `[α, β, γ].eraseVars [0] 1  = [α, γ]`
 -/
-def eraseVars (vs : List Var) (Γ : Context τ) (n : Nat := 0) : Context τ where
-  toList := Γ.toList.eraseAllIdxP (⟨·⟩ ∈ vs) n
+def eraseVars (vs : List Var) (Γ : Context τ) (n : Nat := 0) : Context τ :=
+  let f := fun v Γ => Γ.eraseVar (v + n)
+  vs.foldr f Γ
 
 end Context
